<?xml version="1.0"?>
<rdf:RDF xmlns="http://purl.obolibrary.org/obo/eupath/dev/import_RO.owl#"
     xml:base="http://purl.obolibrary.org/obo/eupath/dev/import_RO.owl"
     xmlns:obo="http://purl.obolibrary.org/obo/"
     xmlns:owl="http://www.w3.org/2002/07/owl#"
     xmlns:rdf="http://www.w3.org/1999/02/22-rdf-syntax-ns#"
     xmlns:xml="http://www.w3.org/XML/1998/namespace"
     xmlns:xsd="http://www.w3.org/2001/XMLSchema#"
     xmlns:rdfs="http://www.w3.org/2000/01/rdf-schema#">
    <owl:Ontology rdf:about="http://purl.obolibrary.org/obo/eupath/dev/import_RO.owl"/>
    


    <!-- 
    ///////////////////////////////////////////////////////////////////////////////////////
    //
    // Annotation properties
    //
    ///////////////////////////////////////////////////////////////////////////////////////
     -->

    


    <!-- http://purl.obolibrary.org/obo/IAO_0000115 -->

    <owl:AnnotationProperty rdf:about="http://purl.obolibrary.org/obo/IAO_0000115"/>
    


    <!-- http://purl.obolibrary.org/obo/IAO_0000118 -->

    <owl:AnnotationProperty rdf:about="http://purl.obolibrary.org/obo/IAO_0000118"/>
    


    <!-- http://purl.obolibrary.org/obo/IAO_0000412 -->

    <owl:AnnotationProperty rdf:about="http://purl.obolibrary.org/obo/IAO_0000412"/>
    


    <!-- 
    ///////////////////////////////////////////////////////////////////////////////////////
    //
    // Object Properties
    //
    ///////////////////////////////////////////////////////////////////////////////////////
     -->

    


    <!-- http://purl.obolibrary.org/obo/BFO_0000050 -->

    <owl:ObjectProperty rdf:about="http://purl.obolibrary.org/obo/BFO_0000050"/>
    


    <!-- http://purl.obolibrary.org/obo/BFO_0000051 -->

    <owl:ObjectProperty rdf:about="http://purl.obolibrary.org/obo/BFO_0000051"/>
    


    <!-- http://purl.obolibrary.org/obo/BFO_0000063 -->

    <owl:ObjectProperty rdf:about="http://purl.obolibrary.org/obo/BFO_0000063"/>
    


    <!-- http://purl.obolibrary.org/obo/RO_0000052 -->

    <owl:ObjectProperty rdf:about="http://purl.obolibrary.org/obo/RO_0000052">
        <rdfs:subPropertyOf rdf:resource="http://purl.obolibrary.org/obo/RO_0002314"/>
        <obo:IAO_0000115 xml:lang="en">a relation between a specifically dependent continuant (the characteristic) and any other entity (the bearer), in which the characteristic depends on the bearer for its existence.</obo:IAO_0000115>
        <obo:IAO_0000412 rdf:resource="http://purl.obolibrary.org/obo/ro.owl"/>
        <rdfs:label xml:lang="en">characteristic of</rdfs:label>
    </owl:ObjectProperty>
    


    <!-- http://purl.obolibrary.org/obo/RO_0000053 -->

    <owl:ObjectProperty rdf:about="http://purl.obolibrary.org/obo/RO_0000053">
        <obo:IAO_0000115 xml:lang="en">Inverse of characteristic_of</obo:IAO_0000115>
        <obo:IAO_0000412 rdf:resource="http://purl.obolibrary.org/obo/ro.owl"/>
        <rdfs:label xml:lang="en">has characteristic</rdfs:label>
    </owl:ObjectProperty>
    


    <!-- http://purl.obolibrary.org/obo/RO_0000056 -->

    <owl:ObjectProperty rdf:about="http://purl.obolibrary.org/obo/RO_0000056">
        <obo:IAO_0000115 xml:lang="en">a relation between a continuant and a process, in which the continuant is somehow involved in the process</obo:IAO_0000115>
        <obo:IAO_0000412 rdf:resource="http://purl.obolibrary.org/obo/ro.owl"/>
        <rdfs:label xml:lang="en">participates in</rdfs:label>
    </owl:ObjectProperty>
    


    <!-- http://purl.obolibrary.org/obo/RO_0000057 -->

    <owl:ObjectProperty rdf:about="http://purl.obolibrary.org/obo/RO_0000057">
        <obo:IAO_0000115 xml:lang="en">a relation between a process and a continuant, in which the continuant is somehow involved in the process</obo:IAO_0000115>
        <obo:IAO_0000412 rdf:resource="http://purl.obolibrary.org/obo/ro.owl"/>
        <rdfs:label xml:lang="en">has participant</rdfs:label>
    </owl:ObjectProperty>
    


    <!-- http://purl.obolibrary.org/obo/RO_0000058 -->

    <owl:ObjectProperty rdf:about="http://purl.obolibrary.org/obo/RO_0000058">
        <obo:IAO_0000115 xml:lang="en">A relationship between a generically dependent continuant and a specifically dependent continuant, in which the generically dependent continuant depends on some independent continuant in virtue of the fact that the specifically dependent continuant also depends on that same independent continuant. A generically dependent continuant may be concretized as multiple specifically dependent continuants.</obo:IAO_0000115>
        <obo:IAO_0000412 rdf:resource="http://purl.obolibrary.org/obo/ro.owl"/>
        <rdfs:label xml:lang="en">is concretized as</rdfs:label>
    </owl:ObjectProperty>
    


    <!-- http://purl.obolibrary.org/obo/RO_0000059 -->

    <owl:ObjectProperty rdf:about="http://purl.obolibrary.org/obo/RO_0000059">
        <obo:IAO_0000115 xml:lang="en">A relationship between a specifically dependent continuant and a generically dependent continuant, in which the generically dependent continuant depends on some independent continuant in virtue of the fact that the specifically dependent continuant also depends on that same independent continuant. Multiple specifically dependent continuants can concretize the same generically dependent continuant.</obo:IAO_0000115>
        <obo:IAO_0000412 rdf:resource="http://purl.obolibrary.org/obo/ro.owl"/>
        <rdfs:label xml:lang="en">concretizes</rdfs:label>
    </owl:ObjectProperty>
    


    <!-- http://purl.obolibrary.org/obo/RO_0000079 -->

    <owl:ObjectProperty rdf:about="http://purl.obolibrary.org/obo/RO_0000079">
        <rdfs:subPropertyOf rdf:resource="http://purl.obolibrary.org/obo/RO_0000052"/>
        <obo:IAO_0000115 xml:lang="en">a relation between a function and an independent continuant (the bearer), in which the function specifically depends on the bearer for its existence</obo:IAO_0000115>
        <obo:IAO_0000412 rdf:resource="http://purl.obolibrary.org/obo/ro.owl"/>
        <rdfs:label xml:lang="en">function of</rdfs:label>
    </owl:ObjectProperty>
    


    <!-- http://purl.obolibrary.org/obo/RO_0000081 -->

    <owl:ObjectProperty rdf:about="http://purl.obolibrary.org/obo/RO_0000081">
        <rdfs:subPropertyOf rdf:resource="http://purl.obolibrary.org/obo/RO_0000052"/>
        <obo:IAO_0000115 xml:lang="en">a relation between a role and an independent continuant (the bearer), in which the role specifically depends on the bearer for its existence</obo:IAO_0000115>
        <obo:IAO_0000412 rdf:resource="http://purl.obolibrary.org/obo/ro.owl"/>
        <rdfs:label xml:lang="en">role of</rdfs:label>
    </owl:ObjectProperty>
    


    <!-- http://purl.obolibrary.org/obo/RO_0000085 -->

    <owl:ObjectProperty rdf:about="http://purl.obolibrary.org/obo/RO_0000085">
        <rdfs:subPropertyOf rdf:resource="http://purl.obolibrary.org/obo/RO_0000053"/>
        <obo:IAO_0000115 xml:lang="en">a relation between an independent continuant (the bearer) and a function, in which the function specifically depends on the bearer for its existence</obo:IAO_0000115>
        <obo:IAO_0000412 rdf:resource="http://purl.obolibrary.org/obo/ro.owl"/>
        <rdfs:label xml:lang="en">has function</rdfs:label>
    </owl:ObjectProperty>
    


    <!-- http://purl.obolibrary.org/obo/RO_0000087 -->

    <owl:ObjectProperty rdf:about="http://purl.obolibrary.org/obo/RO_0000087">
        <rdfs:subPropertyOf rdf:resource="http://purl.obolibrary.org/obo/RO_0000053"/>
        <obo:IAO_0000115 xml:lang="en">a relation between an independent continuant (the bearer) and a role, in which the role specifically depends on the bearer for its existence</obo:IAO_0000115>
        <obo:IAO_0000412 rdf:resource="http://purl.obolibrary.org/obo/ro.owl"/>
        <rdfs:label xml:lang="en">has role</rdfs:label>
    </owl:ObjectProperty>
    


    <!-- http://purl.obolibrary.org/obo/RO_0001000 -->

    <owl:ObjectProperty rdf:about="http://purl.obolibrary.org/obo/RO_0001000">
        <obo:IAO_0000115 xml:lang="en">a relation between two distinct material entities, the new entity and the old entity, in which the new entity begins to exist when the old entity ceases to exist, and the new entity inherits the significant portion of the matter of the old entity</obo:IAO_0000115>
        <obo:IAO_0000412 rdf:resource="http://purl.obolibrary.org/obo/ro.owl"/>
        <rdfs:label xml:lang="en">derives from</rdfs:label>
    </owl:ObjectProperty>
    


    <!-- http://purl.obolibrary.org/obo/RO_0001001 -->

    <owl:ObjectProperty rdf:about="http://purl.obolibrary.org/obo/RO_0001001">
        <obo:IAO_0000115 xml:lang="en">a relation between two distinct material entities, the old entity and the new entity, in which the new entity begins to exist when the old entity ceases to exist, and the new entity inherits the significant portion of the matter of the old entity</obo:IAO_0000115>
        <obo:IAO_0000412 rdf:resource="http://purl.obolibrary.org/obo/ro.owl"/>
        <rdfs:label xml:lang="en">derives into</rdfs:label>
    </owl:ObjectProperty>
    


    <!-- http://purl.obolibrary.org/obo/RO_0001015 -->

    <owl:ObjectProperty rdf:about="http://purl.obolibrary.org/obo/RO_0001015">
        <obo:IAO_0000115 xml:lang="en">a relation between two independent continuants, the location and the target, in which the target is entirely within the location</obo:IAO_0000115>
        <obo:IAO_0000412 rdf:resource="http://purl.obolibrary.org/obo/ro.owl"/>
        <rdfs:label xml:lang="en">location of</rdfs:label>
    </owl:ObjectProperty>
    


    <!-- http://purl.obolibrary.org/obo/RO_0001025 -->

    <owl:ObjectProperty rdf:about="http://purl.obolibrary.org/obo/RO_0001025">
        <obo:IAO_0000115 xml:lang="en">a relation between two independent continuants, the target and the location, in which the target is entirely within the location</obo:IAO_0000115>
        <obo:IAO_0000412 rdf:resource="http://purl.obolibrary.org/obo/ro.owl"/>
        <rdfs:label xml:lang="en">located in</rdfs:label>
    </owl:ObjectProperty>
    


    <!-- http://purl.obolibrary.org/obo/RO_0002081 -->

    <owl:ObjectProperty rdf:about="http://purl.obolibrary.org/obo/RO_0002081">
        <rdfs:subPropertyOf rdf:resource="http://purl.obolibrary.org/obo/RO_0002222"/>
        <obo:IAO_0000412 rdf:resource="http://purl.obolibrary.org/obo/ro.owl"/>
        <rdfs:label xml:lang="en">before or simultaneous with</rdfs:label>
    </owl:ObjectProperty>
    


    <!-- http://purl.obolibrary.org/obo/RO_0002083 -->

    <owl:ObjectProperty rdf:about="http://purl.obolibrary.org/obo/RO_0002083">
        <rdfs:subPropertyOf rdf:resource="http://purl.obolibrary.org/obo/RO_0002081"/>
        <obo:IAO_0000412 rdf:resource="http://purl.obolibrary.org/obo/ro.owl"/>
        <rdfs:label xml:lang="en">before</rdfs:label>
    </owl:ObjectProperty>
    


    <!-- http://purl.obolibrary.org/obo/RO_0002087 -->

    <owl:ObjectProperty rdf:about="http://purl.obolibrary.org/obo/RO_0002087">
        <rdfs:subPropertyOf rdf:resource="http://purl.obolibrary.org/obo/BFO_0000063"/>
        <obo:IAO_0000412 rdf:resource="http://purl.obolibrary.org/obo/ro.owl"/>
        <rdfs:label xml:lang="en">immediately preceded by</rdfs:label>
    </owl:ObjectProperty>
    


    <!-- http://purl.obolibrary.org/obo/RO_0002091 -->

    <owl:ObjectProperty rdf:about="http://purl.obolibrary.org/obo/RO_0002091">
        <rdfs:subPropertyOf rdf:resource="http://purl.obolibrary.org/obo/RO_0002222"/>
        <obo:IAO_0000412 rdf:resource="http://purl.obolibrary.org/obo/ro.owl"/>
        <rdfs:label xml:lang="en">starts during</rdfs:label>
    </owl:ObjectProperty>
    


    <!-- http://purl.obolibrary.org/obo/RO_0002092 -->

    <owl:ObjectProperty rdf:about="http://purl.obolibrary.org/obo/RO_0002092">
        <rdfs:subPropertyOf rdf:resource="http://purl.obolibrary.org/obo/RO_0002091"/>
        <rdfs:subPropertyOf rdf:resource="http://purl.obolibrary.org/obo/RO_0002093"/>
        <obo:IAO_0000412 rdf:resource="http://purl.obolibrary.org/obo/ro.owl"/>
        <rdfs:label xml:lang="en">happens during</rdfs:label>
    </owl:ObjectProperty>
    


    <!-- http://purl.obolibrary.org/obo/RO_0002093 -->

    <owl:ObjectProperty rdf:about="http://purl.obolibrary.org/obo/RO_0002093">
        <rdfs:subPropertyOf rdf:resource="http://purl.obolibrary.org/obo/RO_0002222"/>
        <obo:IAO_0000412 rdf:resource="http://purl.obolibrary.org/obo/ro.owl"/>
        <rdfs:label xml:lang="en">ends during</rdfs:label>
    </owl:ObjectProperty>
    


    <!-- http://purl.obolibrary.org/obo/RO_0002131 -->

    <owl:ObjectProperty rdf:about="http://purl.obolibrary.org/obo/RO_0002131">
        <rdfs:subPropertyOf rdf:resource="http://purl.obolibrary.org/obo/RO_0002323"/>
        <obo:IAO_0000115>x overlaps y if and only if there exists some z such that x has part z and z part of y</obo:IAO_0000115>
        <obo:IAO_0000412 rdf:resource="http://purl.obolibrary.org/obo/ro.owl"/>
        <rdfs:label xml:lang="en">overlaps</rdfs:label>
    </owl:ObjectProperty>
    


    <!-- http://purl.obolibrary.org/obo/RO_0002180 -->

    <owl:ObjectProperty rdf:about="http://purl.obolibrary.org/obo/RO_0002180">
        <rdfs:subPropertyOf rdf:resource="http://purl.obolibrary.org/obo/BFO_0000051"/>
        <obo:IAO_0000115>w &apos;has component&apos; p if w &apos;has part&apos; p and w is such that it can be directly disassembled into into n parts p, p2, p3, ..., pn, where these parts are of similar type.</obo:IAO_0000115>
        <obo:IAO_0000412 rdf:resource="http://purl.obolibrary.org/obo/ro.owl"/>
        <rdfs:label xml:lang="en">has component</rdfs:label>
    </owl:ObjectProperty>
    


    <!-- http://purl.obolibrary.org/obo/RO_0002215 -->

    <owl:ObjectProperty rdf:about="http://purl.obolibrary.org/obo/RO_0002215">
        <rdfs:subPropertyOf rdf:resource="http://purl.obolibrary.org/obo/RO_0002216"/>
        <obo:IAO_0000115>A relation between a material entity (such as a cell) and a process, in which the material entity has the ability to carry out the process. </obo:IAO_0000115>
        <obo:IAO_0000412 rdf:resource="http://purl.obolibrary.org/obo/ro.owl"/>
        <rdfs:label xml:lang="en">capable of</rdfs:label>
    </owl:ObjectProperty>
    


    <!-- http://purl.obolibrary.org/obo/RO_0002216 -->

    <owl:ObjectProperty rdf:about="http://purl.obolibrary.org/obo/RO_0002216">
        <rdfs:subPropertyOf rdf:resource="http://purl.obolibrary.org/obo/RO_0002328"/>
        <rdfs:subPropertyOf rdf:resource="http://purl.obolibrary.org/obo/RO_0002500"/>
        <obo:IAO_0000115>c stands in this relationship to p if and only if there exists some p&apos; such that c is capable_of p&apos;, and p&apos; is part_of p.</obo:IAO_0000115>
        <obo:IAO_0000412 rdf:resource="http://purl.obolibrary.org/obo/ro.owl"/>
        <rdfs:label xml:lang="en">capable of part of</rdfs:label>
    </owl:ObjectProperty>
    


    <!-- http://purl.obolibrary.org/obo/RO_0002222 -->

    <owl:ObjectProperty rdf:about="http://purl.obolibrary.org/obo/RO_0002222">
        <obo:IAO_0000412 rdf:resource="http://purl.obolibrary.org/obo/ro.owl"/>
        <rdfs:label xml:lang="en">temporally related to</rdfs:label>
    </owl:ObjectProperty>
    


    <!-- http://purl.obolibrary.org/obo/RO_0002223 -->

    <owl:ObjectProperty rdf:about="http://purl.obolibrary.org/obo/RO_0002223">
        <rdfs:subPropertyOf rdf:resource="http://purl.obolibrary.org/obo/BFO_0000050"/>
        <rdfs:subPropertyOf rdf:resource="http://purl.obolibrary.org/obo/RO_0002222"/>
        <obo:IAO_0000115>inverse of starts with</obo:IAO_0000115>
        <obo:IAO_0000412 rdf:resource="http://purl.obolibrary.org/obo/ro.owl"/>
        <rdfs:label xml:lang="en">starts</rdfs:label>
    </owl:ObjectProperty>
    


    <!-- http://purl.obolibrary.org/obo/RO_0002248 -->

    <owl:ObjectProperty rdf:about="http://purl.obolibrary.org/obo/RO_0002248">
        <rdfs:subPropertyOf rdf:resource="http://purl.obolibrary.org/obo/BFO_0000051"/>
        <obo:IAO_0000115>A relationship that holds between a substance and a chemical entity, if the chemical entity is part of the substance, and the chemical entity forms the biologically active component of the substance.</obo:IAO_0000115>
        <obo:IAO_0000118>has active pharmaceutical ingredient</obo:IAO_0000118>
        <obo:IAO_0000118>has active substance</obo:IAO_0000118>
        <obo:IAO_0000412 rdf:resource="http://purl.obolibrary.org/obo/ro.owl"/>
        <rdfs:label>has active ingredient</rdfs:label>
    </owl:ObjectProperty>
    


    <!-- http://purl.obolibrary.org/obo/RO_0002249 -->

    <owl:ObjectProperty rdf:about="http://purl.obolibrary.org/obo/RO_0002249">
        <rdfs:subPropertyOf rdf:resource="http://purl.obolibrary.org/obo/BFO_0000050"/>
        <obo:IAO_0000115>inverse of has active ingredient</obo:IAO_0000115>
        <obo:IAO_0000412 rdf:resource="http://purl.obolibrary.org/obo/ro.owl"/>
        <rdfs:label>active ingredient in</rdfs:label>
    </owl:ObjectProperty>
    


    <!-- http://purl.obolibrary.org/obo/RO_0002314 -->

    <owl:ObjectProperty rdf:about="http://purl.obolibrary.org/obo/RO_0002314">
        <rdfs:subPropertyOf rdf:resource="http://purl.obolibrary.org/obo/RO_0002502"/>
        <obo:IAO_0000115>q characteristic of part of w if and only if there exists some p such that q inheres in p and p part of w.</obo:IAO_0000115>
        <obo:IAO_0000412 rdf:resource="http://purl.obolibrary.org/obo/ro.owl"/>
        <rdfs:label xml:lang="en">characteristic of part of</rdfs:label>
    </owl:ObjectProperty>
    


    <!-- http://purl.obolibrary.org/obo/RO_0002323 -->

    <owl:ObjectProperty rdf:about="http://purl.obolibrary.org/obo/RO_0002323">
        <obo:IAO_0000115>A mereological relationship or a topological relationship</obo:IAO_0000115>
        <obo:IAO_0000412 rdf:resource="http://purl.obolibrary.org/obo/ro.owl"/>
        <rdfs:label xml:lang="en">mereotopologically related to</rdfs:label>
    </owl:ObjectProperty>
    


    <!-- http://purl.obolibrary.org/obo/RO_0002328 -->

    <owl:ObjectProperty rdf:about="http://purl.obolibrary.org/obo/RO_0002328">
        <obo:IAO_0000115>A grouping relationship for any relationship directly involving a function, or that holds because of a function of one of the related entities.</obo:IAO_0000115>
        <obo:IAO_0000412 rdf:resource="http://purl.obolibrary.org/obo/ro.owl"/>
        <rdfs:label xml:lang="en">functionally related to</rdfs:label>
    </owl:ObjectProperty>
    


    <!-- http://purl.obolibrary.org/obo/RO_0002351 -->

    <owl:ObjectProperty rdf:about="http://purl.obolibrary.org/obo/RO_0002351">
        <rdfs:subPropertyOf rdf:resource="http://purl.obolibrary.org/obo/BFO_0000051"/>
        <obo:IAO_0000115>has member is a mereological relation between a collection and an item.</obo:IAO_0000115>
        <obo:IAO_0000412 rdf:resource="http://purl.obolibrary.org/obo/ro.owl"/>
        <rdfs:label xml:lang="en">has member</rdfs:label>
    </owl:ObjectProperty>
    


    <!-- http://purl.obolibrary.org/obo/RO_0002410 -->

    <owl:ObjectProperty rdf:about="http://purl.obolibrary.org/obo/RO_0002410">
        <obo:IAO_0000115>relation that links two events, processes, states, or objects such that one event, process, state, or object (a cause) contributes to the production of another event, process, state, or object (an effect) where the cause is partly or wholly responsible for the effect, and the effect is partly or wholly dependent on the cause.</obo:IAO_0000115>
        <obo:IAO_0000412 rdf:resource="http://purl.obolibrary.org/obo/ro.owl"/>
        <rdfs:label xml:lang="en">causally related to</rdfs:label>
    </owl:ObjectProperty>
    


    <!-- http://purl.obolibrary.org/obo/RO_0002418 -->

    <owl:ObjectProperty rdf:about="http://purl.obolibrary.org/obo/RO_0002418">
        <rdfs:subPropertyOf rdf:resource="http://purl.obolibrary.org/obo/RO_0002501"/>
        <obo:IAO_0000115>p is &apos;causally upstream or within&apos; q iff p is causally related to q, and the end of p precedes, or is coincident with, the end of q.</obo:IAO_0000115>
        <obo:IAO_0000118>affects</obo:IAO_0000118>
        <obo:IAO_0000412 rdf:resource="http://purl.obolibrary.org/obo/ro.owl"/>
        <rdfs:label>causally upstream of or within</rdfs:label>
    </owl:ObjectProperty>
    


    <!-- http://purl.obolibrary.org/obo/RO_0002500 -->

    <owl:ObjectProperty rdf:about="http://purl.obolibrary.org/obo/RO_0002500">
        <rdfs:subPropertyOf rdf:resource="http://purl.obolibrary.org/obo/RO_0002595"/>
        <obo:IAO_0000115>A relationship between a material entity and a process where the material entity has some causal role that influences the process</obo:IAO_0000115>
        <obo:IAO_0000412 rdf:resource="http://purl.obolibrary.org/obo/ro.owl"/>
        <rdfs:label>causal agent in process</rdfs:label>
    </owl:ObjectProperty>
    


    <!-- http://purl.obolibrary.org/obo/RO_0002501 -->

    <owl:ObjectProperty rdf:about="http://purl.obolibrary.org/obo/RO_0002501">
        <rdfs:subPropertyOf rdf:resource="http://purl.obolibrary.org/obo/RO_0002410"/>
        <obo:IAO_0000115>p is causally related to q if and only if p or any part of p and q or any part of q are linked by a chain of events where each event pair is one where the execution of p influences the execution of q. p may be upstream, downstream, part of, or a container of q.</obo:IAO_0000115>
        <obo:IAO_0000412 rdf:resource="http://purl.obolibrary.org/obo/ro.owl"/>
        <rdfs:label>causal relation between processes</rdfs:label>
    </owl:ObjectProperty>
    


    <!-- http://purl.obolibrary.org/obo/RO_0002502 -->

    <owl:ObjectProperty rdf:about="http://purl.obolibrary.org/obo/RO_0002502">
        <obo:IAO_0000412 rdf:resource="http://purl.obolibrary.org/obo/ro.owl"/>
        <rdfs:label>depends on</rdfs:label>
    </owl:ObjectProperty>
    


    <!-- http://purl.obolibrary.org/obo/RO_0002595 -->

    <owl:ObjectProperty rdf:about="http://purl.obolibrary.org/obo/RO_0002595">
        <rdfs:subPropertyOf rdf:resource="http://purl.obolibrary.org/obo/RO_0002410"/>
        <obo:IAO_0000115>A relationship that holds between a material entity and a process in which causality is involved, with either the material entity or some part of the material entity exerting some influence over the process, or the process influencing some aspect of the material entity.</obo:IAO_0000115>
        <obo:IAO_0000412 rdf:resource="http://purl.obolibrary.org/obo/ro.owl"/>
        <rdfs:label>causal relation between material entity and a process</rdfs:label>
    </owl:ObjectProperty>
    


    <!-- http://purl.obolibrary.org/obo/RO_0002606 -->

    <owl:ObjectProperty rdf:about="http://purl.obolibrary.org/obo/RO_0002606">
        <rdfs:subPropertyOf rdf:resource="http://purl.obolibrary.org/obo/RO_0002410"/>
        <obo:IAO_0000115>c is a substance that treats d if c is a material entity (such as a small molecule or compound) and d is a pathological process, phenotype or disease, and c is capable of some activity that negative regulates or decreases the magnitude of d.</obo:IAO_0000115>
        <obo:IAO_0000412 rdf:resource="http://purl.obolibrary.org/obo/ro.owl"/>
        <rdfs:label>is substance that treats</rdfs:label>
    </owl:ObjectProperty>
</rdf:RDF>



<!-- Generated by the OWL API (version 4.5.6) https://github.com/owlcs/owlapi -->

